silveroak-opentitan/hmac/end2end/RunSha256SoftwareOnCava.v
@@ -11,10 +11,6 @@ Require Import riscv.Spec.Decode.
 Require Import riscv.Utility.InstructionCoercions.
 Open Scope ilist_scope.
 
-Definition all_insts: list Instruction :=
-  sha256_example_asm ++ [[ Jal RegisterNames.ra
-            (main_relative_pos + word.signed (word.sub code_start p_call))]].
-
 Definition test_msg_str: string := "Hello world".
 
 Definition test_msg: list Byte.byte := Eval compute in list_byte_of_string test_msg_str.
@@ -24,34 +20,43 @@ Definition expected_output: list Byte.byte := [
   Byte.x64; Byte.xec; Byte.x88; Byte.xca; Byte.x00; Byte.xb2; Byte.x68; Byte.xe5; Byte.xba; Byte.x1a; Byte.x35; Byte.x67; Byte.x8a; Byte.x1b; Byte.x53; Byte.x16; Byte.xd2; Byte.x12; Byte.xf4; Byte.xf3; Byte.x66; Byte.xb2; Byte.x47; Byte.x72; Byte.x32; Byte.x53; Byte.x4a; Byte.x8a; Byte.xec; Byte.xa3; Byte.x7f; Byte.x3c
 ].
 
-Definition digest_loc  : Z := word.unsigned heap_start + 12.
+Definition code_start    : word := word.of_Z 0.
+Definition code_pastend  : word := word.of_Z (4*2^10).
+Definition heap_start    : word := word.of_Z (4*2^10).
+Definition heap_pastend  : word := word.of_Z (8*2^10).
+Definition stack_start   : word := word.of_Z (8*2^10).
+Definition stack_pastend : word := word.of_Z (16*2^10).
+
+Definition digest_loc  : Z := word.unsigned heap_start.
 Definition digest_len  : Z := 256/8.
 Definition msg_loc     : Z := digest_loc + digest_len.
 Definition msg_len     : Z := Z.of_nat (List.length test_msg).
-Definition msg_len_loc : Z := msg_loc + msg_len.
 
 (* just some pattern of the right length, easy to spot while debugging: *)
 Definition initial_data_at_digest: list Byte.byte :=
   [Byte.xaa] ++ (List.repeat Byte.xbb (Z.to_nat digest_len - 2)) ++ [Byte.xcc].
 
+(* Invalid ra, will cause crash (intended), but in real usage, this would be a
+   return address pointing into the caller's code. *)
+Definition ret_addr: word := word.of_Z (-4).
+
 Definition initial_def: ExtraRiscvMachine hmac_device := {|
   getMachine := {|
-    getRegs := map.put (map.of_list (List.map (fun n => (Z.of_nat n, word.of_Z 0)) (List.seq 0 32)))
-                       RegisterNames.sp stack_pastend;
-    getPc := p_call;
-    getNextPc := word.add p_call (word.of_Z 4);
-    getMem := (map.putmany (map.of_list_word_at code_start (Pipeline.instrencode all_insts))
+    getRegs := map.put (map.put (map.put (map.put (map.put
+      (map.of_list (List.map (fun n => (Z.of_nat n, word.of_Z 0)) (List.seq 0 32)))
+      RegisterNames.sp stack_pastend)
+      RegisterNames.a0 (word.of_Z digest_loc))
+      RegisterNames.a1 (word.of_Z msg_loc))
+      RegisterNames.a2 (word.of_Z msg_len))
+      RegisterNames.ra ret_addr;
+    getPc := word.add code_start (word.of_Z sha256_relative_pos);
+    getNextPc := word.add (word.add code_start (word.of_Z sha256_relative_pos)) (word.of_Z 4);
+    getMem := (map.putmany (map.of_list_word_at code_start (Pipeline.instrencode sha256_asm))
               (map.putmany (map.of_list_word_at (word.sub stack_pastend (word.of_Z 512))
                                                 (List.repeat Byte.x00 512))
-              (map.of_list_word_at heap_start
-                        (HList.tuple.to_list (LittleEndian.split 4 digest_loc) ++
-                         HList.tuple.to_list (LittleEndian.split 4 msg_loc) ++
-                         HList.tuple.to_list (LittleEndian.split 4 msg_len_loc) ++
-                         initial_data_at_digest ++
-                         test_msg ++
-                         HList.tuple.to_list (LittleEndian.split 4 msg_len)))));
+              (map.of_list_word_at heap_start (initial_data_at_digest ++ test_msg))));
     getXAddrs := List.map (fun n => word.add code_start (word.of_Z (Z.of_nat n)))
-                          (List.seq 0 (4 * List.length all_insts));
+                          (List.seq 0 (4 * List.length sha256_asm));
     getLog := [];
   |};
   getExtraState := tt; (* TODO replace by reset_state *)
@@ -100,9 +105,9 @@ Compute (snd (fst sha256_compile_result)).
 Compute snd (trace 50 initial).
 *)
 
-Definition res(nsteps: nat): LogElem := outcomeToLogElem (run sched nsteps initial).
+Definition res(nsteps: nat): LogElem := outcomeToLogElem (run_rec sched 0 nsteps initial).
 
-Goal exists nsteps, res nsteps = (true, word.unsigned p_call + 4, expected_output).
+Goal exists nsteps, res nsteps = (true, word.unsigned ret_addr, expected_output).
   (* wrong number of steps, and doesn't work currently because Cava Hmac device is not yet
      hooked up, and probably there are also bugs in the Hmac driver code and in the current file *)
   exists 20%nat. vm_compute. (* `reflexivity` is supposed to work here eventually *)
